ulib/experimental/Steel.HigherReference.fst
@@ -1,0 +1,409 @@
+module Steel.HigherReference
+
+open Steel.Actions
+open Steel.SteelAtomic.Basics
+module Sem = Steel.Semantics.Hoare.MST
+
+#push-options "--fuel 0 --ifuel 1"
+let alloc (#a:Type) (x:a)
+  : SteelT (ref a) emp (fun r -> pts_to r full x)
+  = Steel?.reflect (fun _ ->
+      let m0 = mst_get () in
+      let act = alloc_ref x trivial_preorder in
+      let (| x, m1 |) = act m0 in
+      act_preserves_frame_and_preorder act m0;
+      mst_put m1;
+      x)
+
+let read_core (#a:Type) (#uses:Set.set lock_addr) (#p:perm) (r:ref a)
+  : SteelAtomic a uses false (ref_perm r p) (fun x -> pts_to r p x)
+  = SteelAtomic?.reflect (fun _ ->
+      let m0 = mst_get () in
+      let act = get_ref uses r p in
+      let (| x, m1 |) = act m0 in
+      atomic_preserves_frame_and_preorder act m0;
+      mst_put m1;
+      x)
+
+
+let read_atomic (#a:Type) (#uses:Set.set lock_addr) (#p:perm) (#v:erased a) (r:ref a)
+  : SteelAtomic a uses false (pts_to r p v) (fun x -> pts_to r p x)
+  = change_hprop (pts_to r p v) (ref_perm r p) (fun m -> intro_exists v (pts_to_ref r p) m);
+    read_core r
+
+let read (#a:Type) (#p:perm) (#v:erased a) (r:ref a)
+  : SteelT a (pts_to r p v) (fun x -> pts_to r p x)
+  = lift_atomic_to_steelT (fun _ -> read_atomic r)
+
+let read_refine_core_atomic (#a:Type) (#uses:Set.set lock_addr) (#p:perm) (q:a -> hprop) (r:ref a)
+  : SteelAtomic a uses false
+    (h_exists (fun (v:a) -> pts_to_ref r p v `star` q v))
+    (fun x -> pts_to_ref r p x `star` q x)
+  = SteelAtomic?.reflect (fun _ ->
+      let m0 = mst_get () in
+      let act = get_ref_refine uses r p q in
+      let (| x, m1 |) = act m0 in
+      atomic_preserves_frame_and_preorder act m0;
+      mst_put m1;
+      x)
+
+let read_refine_atomic (#a:Type) (#uses:Set.set lock_addr) (#p:perm) (q:a -> hprop) (r:ref a)
+  : SteelAtomic a uses false
+    (h_exists (fun (v:a) -> pts_to r p v `star` q v))
+    (fun x -> pts_to r p x `star` q x)
+  = change_hprop
+      (h_exists (fun (v:a) -> pts_to r p v `star` q v))
+      (h_exists (fun (v:a) -> pts_to_ref r p v `star` q v))
+      (fun m -> h_exists_extensionality
+        (fun (v:a) -> pts_to r p v `star` q v)
+        (fun (v:a) -> pts_to_ref r p v `star` q v)
+      );
+    let x = read_refine_core_atomic q r in
+    change_hprop (pts_to_ref r p x `star` q x) (pts_to r p x `star` q x) (fun m -> ());
+    return_atomic x
+
+let read_refine (#a:Type) (#p:perm) (q:a -> hprop) (r:ref a)
+  : SteelT a (h_exists (fun (v:a) -> pts_to r p v `star` q v))
+             (fun v -> pts_to r p v `star` q v)
+  = lift_atomic_to_steelT (fun _ -> read_refine_atomic q r)
+
+let write_atomic (#a:Type) (#uses:Set.set lock_addr) (#v:erased a) (r:ref a) (x:a)
+  : SteelAtomic unit uses false (pts_to r full v) (fun _ -> pts_to r full x)
+  = SteelAtomic?.reflect (fun _ ->
+      let m0 = mst_get () in
+      let act = set_ref uses r v x in
+      let (| x, m1 |) = act m0 in
+      atomic_preserves_frame_and_preorder act m0;
+      mst_put m1;
+      x)
+
+let write (#a:Type) (#v:erased a) (r:ref a) (x:a)
+  : SteelT unit (pts_to r full v) (fun _ -> pts_to r full x)
+  = lift_atomic_to_steelT (fun _ -> write_atomic r x)
+
+let free_core (#a:Type) (r:ref a)
+  : SteelT unit (ref_perm r full) (fun _ -> emp)
+  = Steel?.reflect (fun _ ->
+      let m0 = mst_get () in
+      let act = free_ref r in
+      let (| x, m1 |) = act m0 in
+      act_preserves_frame_and_preorder act m0;
+      mst_put m1;
+      x)
+
+let free (#a:Type) (#v:erased a) (r:ref a)
+  : SteelT unit (pts_to r full v) (fun _ -> emp)
+  = lift_atomic_to_steelT (fun _ -> change_hprop (pts_to r full v) (ref_perm r full) (fun m -> intro_exists v (pts_to_ref r full) m));
+    free_core r
+
+let share_atomic (#a:Type) (#uses:Set.set lock_addr) (#p:perm) (#v:erased a) (r:ref a)
+  : SteelAtomic unit
+    uses
+    true
+    (pts_to r p v)
+    (fun _ -> pts_to r (half_perm p) v `star` pts_to r (half_perm p) v)
+  = change_hprop
+      (pts_to r p v)
+      (pts_to r (half_perm p) v `star` pts_to r (half_perm p) v)
+      (fun m -> share_pts_to_ref r p v m)
+
+let share (#a:Type) (#p:perm) (#v:erased a) (r:ref a)
+  : SteelT unit
+    (pts_to r p v)
+    (fun _ -> pts_to r (half_perm p) v `star` pts_to r (half_perm p) v)
+  = lift_atomic_to_steelT (fun _ -> share_atomic r)
+
+let gather_atomic
+  (#a:Type) (#uses:Set.set lock_addr)
+  (#p0:perm) (#p1:perm) (#v0 #v1:erased a) (r:ref a)
+  : SteelAtomic unit
+    uses
+    true
+    (pts_to r p0 v0 `star` pts_to r p1 v1)
+    (fun _ -> pts_to r (sum_perm p0 p1) v0)
+  = change_hprop
+      (pts_to r p0 v0 `star` pts_to r p1 v1)
+      (pts_to r (sum_perm p0 p1) v0)
+      (fun m -> gather_pts_to_ref r p0 p1 v0 v1 m)
+
+let gather (#a:Type) (#p0:perm) (#p1:perm) (#v0 #v1:erased a) (r:ref a)
+  : SteelT unit
+    (pts_to r p0 v0 `star` pts_to r p1 v1)
+    (fun _ -> pts_to r (sum_perm p0 p1) v0)
+  = lift_atomic_to_steelT (fun _ -> gather_atomic r)
+
+let ghost_read (#a:Type) (#uses:Set.set lock_addr) (#p:perm) (#v:Ghost.erased a) (r:ref a)
+  : SteelAtomic a uses true
+    (pts_to r p v)
+    (fun x -> pts_to r p x)
+  = SteelAtomic?.reflect (fun _ ->
+      let m0 = mst_get () in
+      // TODO: Needs to expose such an action. The ref should probably be to Ghost.erased a
+      admit())
+
+let ghost_read_refine (#a:Type) (#uses:Set.set lock_addr) (#p:perm) (r:ref a)
+  (q:a -> hprop)
+  : SteelAtomic a uses true
+    (h_exists (fun (v:a) -> pts_to r p v `star` q v))
+    (fun v -> pts_to r p v `star` q v)
+  = SteelAtomic?.reflect (fun _ ->
+      let m0 = mst_get () in
+      // TODO: Needs to expose such an action. The ref should probably be to Ghost.erased a
+      admit())
+
+
+
+let alloc_monotonic_ref = admit()
+let read_monotonic_ref = admit()
+let write_monotonic_ref = admit()
+
+let pure (p:prop) : hprop =
+ refine emp (fun _ -> p)
+
+#set-options "--print_universes --print_implicits"
+
+let witnessed
+  (#t:Type u#1)
+  (#p:Preorder.preorder t)
+  (r:reference t p)
+  (fact:property t)
+              =
+  RMST.witnessed mem mem_evolves (fun (m: mem) ->
+    (interp (ref_or_dead r) m /\ fact (sel_ref_or_dead r m))
+  )
+
+#restart-solver
+
+let ac_reasoning_for_witness_atomic (p q: hprop) (f: prop) : Lemma
+  (requires f)
+  (ensures (p `equiv` (p `star` pure f)))
+  =
+  calc (equiv) {
+    p;
+    (equiv) {emp_unit p}
+    (p `star` emp);
+    (equiv) {star_commutative p emp}
+    (emp `star` p);
+    (equiv) {
+      let aux (h: mem) : Lemma (
+        (interp (emp `star` p) h /\ f) <==>
+        (interp (refine (emp `star` p) (fun _ -> f)) h)
+      ) =
+        refine_equiv (emp `star` p) (fun _ -> f) h
+      in
+      Classical.forall_intro aux
+    }
+    (refine (emp `star` p) (fun _ -> f));
+    (equiv) { refine_star emp p (fun _ -> f)}
+    (refine emp (fun _ -> f) `star` p);
+    (equiv) { () }
+    (pure f `star` p);
+    (equiv) { star_commutative (pure f) p }
+    (p `star` pure f);
+  }
+
+
+let ac_reasoning_for_frame_on_noop
+  (p q r s: hprop)
+  (m :mem)
+  : Lemma
+    (requires ((p `equiv` q) /\
+      interp ((p `star` r) `star` s) m
+    ))
+    (ensures (interp ((q `star` r) `star` s)) m)
+  =
+  star_associative p r s;
+  equiv_extensional_on_star p q (r `star` s);
+  assert(interp (q `star` (r `star` s)) m);
+  star_associative q r s
+
+#push-options "--fuel 2 --ifuel 1"
+let preserves_frame_on_noop
+  (uses:Set.set lock_addr)
+  (#st: Sem.st{st == state_uses uses})
+  (pre post: st.Sem.hprop)
+  (m: st.Sem.mem)
+  : Lemma
+    (requires (forall (m: st.Sem.mem). st.Sem.interp pre m <==> st.Sem.interp post m))
+    (ensures (Sem.preserves_frame pre post m m))
+  =
+   let aux (frame:st.Sem.hprop) : Lemma (
+    st.Sem.interp ((pre `st.Sem.star` frame) `st.Sem.star` (st.Sem.locks_invariant m)) m ==>
+    (st.Sem.interp ((post `st.Sem.star` frame) `st.Sem.star` (st.Sem.locks_invariant m)) m /\
+     (forall (f_frame:Sem.fp_prop frame). f_frame (st.Sem.core m) == f_frame (st.Sem.core m))))
+   =
+     let aux (_ :squash (
+       st.Sem.interp ((pre `st.Sem.star` frame) `st.Sem.star` (st.Sem.locks_invariant m)) m
+     )) : Lemma (
+       (st.Sem.interp ((post `st.Sem.star` frame) `st.Sem.star` (st.Sem.locks_invariant m)) m /\
+       (forall (f_frame:Sem.fp_prop frame). f_frame (st.Sem.core m) == f_frame (st.Sem.core m)))
+     ) =
+       ac_reasoning_for_frame_on_noop pre post frame (st.Sem.locks_invariant m) m
+     in
+     Classical.impl_intro aux
+   in
+   Classical.forall_intro aux
+#pop-options
+
+#push-options "--fuel 0 --ifuel 0 --z3rlimit 10"
+let witness_atomic
+  (#a:Type)
+  (#uses:Set.set lock_addr)
+  (#q:perm)
+  (#p:Preorder.preorder a)
+  (r:reference a p)
+  (fact:stable_property p)
+  (v:(Ghost.erased a))
+  (_:squash (fact v))
+  : SteelAtomic unit uses true
+    (pts_to_ref r q v)
+    (fun _ -> pts_to_ref r q v `star` pure (witnessed r fact))
+  =
+  SteelAtomic?.reflect (fun _ ->
+   let m0 = mst_get () in
+   intro_exists v (pts_to_ref r q) m0;
+   sel_ref_lemma r q m0;
+   pts_to_ref_injective r q v (sel_ref r m0) m0;
+   let fact_mem : RMST.s_predicate mem = (fun m ->
+    interp (ref_or_dead r) m /\ fact (sel_ref_or_dead r m)
+   ) in
+   let aux (m0 m1: mem) : Lemma ((fact_mem m0 /\ mem_evolves m0 m1) ==> fact_mem m1) =
+     let aux (_ :squash (fact_mem m0 /\ mem_evolves m0 m1)) : Lemma (fact_mem m1) =
+       reference_preorder_respected r m0 m1
+     in
+     Classical.impl_intro aux
+   in
+   Classical.forall_intro_2 aux;
+   assert(RMST.stable mem mem_evolves fact_mem);
+   sel_ref_or_dead_lemma r m0;
+   RMST.witness mem mem_evolves fact_mem;
+   let m1 = mst_get () in
+   assert(m0 == m1);
+   ac_reasoning_for_witness_atomic
+     (pts_to_ref r q v)
+     (locks_invariant uses m1)
+     (witnessed r fact);
+   equiv_extensional_on_star
+     (pts_to_ref r q v)
+     ((pts_to_ref r q v) `star` pure (witnessed r fact))
+     (locks_invariant uses m1);
+   let aux (m: mem) : Lemma(
+     interp (pts_to_ref r q v) m <==> interp (pts_to_ref r q v `star` pure (witnessed r fact)) m
+   ) =
+     let aux (_ : squash (interp (pts_to_ref r q v) m)) : Lemma (
+       interp (pts_to_ref r q v `star` pure (witnessed r fact)) m
+     ) =
+       ac_reasoning_for_witness_atomic (pts_to_ref r q v) emp (witnessed r fact)
+     in
+     Classical.impl_intro aux;
+     let aux (_ : squash (interp (pts_to_ref r q v `star` pure (witnessed r fact)) m)) : Lemma (
+       interp (pts_to_ref r q v) m
+     ) =
+       affine_star (pts_to_ref r q v) (pure (witnessed r fact)) m
+     in
+     Classical.impl_intro aux
+   in
+   Classical.forall_intro aux;
+   preserves_frame_on_noop
+     uses
+     #(state_uses uses)
+     (pts_to_ref r q v)
+     (pts_to_ref r q v `star` pure (witnessed r fact))
+     m0
+  )
+#pop-options
+
+let witness (#a:Type) (#q:perm) (#p:Preorder.preorder a) (r:reference a p)
+            (fact:stable_property p)
+            (v:(Ghost.erased a))
+            (pf:squash (fact v))
+  : SteelT unit (pts_to_ref r q v)
+                (fun _ -> pts_to_ref r q v `star` pure (witnessed r fact))
+  =
+  lift_atomic_to_steelT (fun _ -> witness_atomic r fact v pf)
+
+let ac_reasoning_for_recall_atomic (p: hprop) (f: prop) (m: mem) : Lemma
+  (requires (interp (p `star` pure f)) m)
+  (ensures (f))
+  =
+  affine_star p (pure f) m;
+  refine_equiv emp (fun _ -> f) m
+
+let mst_admit (#a:Type) ()
+: Mst a (fun _ -> True) (fun _ _ _ -> False)
+= RMST.rmst_admit ()
+
+#push-options "--fuel 0 --ifuel 0 --z3rlimit 10"
+let recall_atomic
+  (#a:Type)
+  (#uses:Set.set lock_addr)
+  (#q:perm)
+  (#p:Preorder.preorder a)
+  (#fact:property a)
+  (r:reference a p)
+  (v:(Ghost.erased a))
+  : SteelAtomic unit uses true
+    (pts_to_ref r q v `star` pure (witnessed r fact))
+    (fun _ -> pts_to_ref r q v `star` pure (fact v))
+  = SteelAtomic?.reflect (fun _ ->
+   let m0 = mst_get () in
+   intro_exists v (pts_to_ref r q) m0;
+   sel_ref_lemma r q m0;
+   pts_to_ref_injective r q v (sel_ref r m0) m0;
+   ac_reasoning_for_recall_atomic (pts_to_ref r q v) (witnessed r fact) m0;
+   let fact_mem : RMST.s_predicate mem = (fun m ->
+    interp (ref_or_dead r) m /\ fact (sel_ref_or_dead r m)
+   ) in
+   RMST.recall mem mem_evolves fact_mem;
+   let m1 = mst_get () in
+   assert(m0 == m1);
+   sel_ref_or_dead_lemma r m1;
+   assert(Ghost.reveal v == sel_ref r m1);
+   assert(Ghost.reveal v == sel_ref_or_dead r m1);
+   assert(fact (Ghost.reveal v));
+   let aux (m: mem) : Lemma(
+     interp (pts_to_ref r q v `star` pure (witnessed r fact)) m <==>
+     interp (pts_to_ref r q v `star` pure (fact v)) m
+   ) =
+     let aux (_ : squash (interp (pts_to_ref r q v `star` pure (fact v)) m)) : Lemma (
+       interp (pts_to_ref r q v `star` pure (witnessed r fact)) m
+     ) =
+       affine_star (pts_to_ref r q v) (pure (fact v)) m1;
+       ac_reasoning_for_witness_atomic (pts_to_ref r q v) emp (witnessed r fact)
+     in
+     Classical.impl_intro aux;
+     let aux (_ : squash (interp (pts_to_ref r q v `star` pure (witnessed r fact)) m)) : Lemma (
+       interp (pts_to_ref r q v `star` pure (fact v)) m
+     ) =
+       affine_star (pts_to_ref r q v) (pure (witnessed r fact)) m;
+       ac_reasoning_for_witness_atomic (pts_to_ref r q v) emp (fact v)
+     in
+     Classical.impl_intro aux
+   in
+   Classical.forall_intro aux;
+   preserves_frame_on_noop
+     uses
+     #(state_uses uses)
+     (pts_to_ref r q v `star` pure (witnessed r fact))
+     (pts_to_ref r q v `star` pure (fact v))
+     m0;
+
+   assert (interp ((pts_to_ref r q v `star` pure (witnessed r fact)) `star` (locks_invariant uses m1)) m1);
+   assert (equiv (pts_to_ref r q v `star` pure (witnessed r fact))
+                 (pts_to_ref r q v `star` pure (fact v)));
+
+   equiv_extensional_on_star (pts_to_ref r q v `star` pure (witnessed r fact))
+                             (pts_to_ref r q v `star` pure (fact v))
+                             (locks_invariant uses m1);
+   assert (interp ((pts_to_ref r q v `star` pure (fact v)) `star` (locks_invariant uses m1)) m1)
+ )
+#pop-options
+
+
+let recall (#a:Type) (#q:perm) (#p:Preorder.preorder a) (#fact:property a)
+           (r:reference a p) (v:(Ghost.erased a))
+  : SteelT unit (pts_to_ref r q v `star` pure (witnessed r fact))
+                (fun _ -> pts_to_ref r q v `star` pure (fact v))
+
+  =
+  lift_atomic_to_steelT (fun _ -> recall_atomic r v)
